\section{The Riemann Integral}

\begin{definition}
Let $I = [a, b]$, where $a$ and $b$ are real numbers, be a subset of $\mathbb{R}$ and let 
\begin{align*}
    P = \{x_{0}, x_{1}, x_{2}, ..., x_{n-1}, x_{n}\} \hspace{20pt} \text{such that} \hspace{20pt} a = x_{0} < x_{1} < x_{2} < \cdots < x_{n-1} < x_{n} = b
\end{align*}
be a finite subset of numbers contained in $I$. Take each member $x_{i}$ of $P$ and use it to create a sub-interval $I_{i}$ of $I$, such that the union of these sub-intervals is $I$, as follows
\begin{align*}
    I_{0} = [x_{0}, x_{1}) \hspace{20pt} I_{1} = [x_{1}, x_{2})& \hspace{20pt} \cdots \hspace{20pt} I_{n-2} = [x_{n-2}, x_{n-1}) \hspace{20pt} I_{n-1} = [x_{n-1}, x_{n}]\\[2ex]
    &I = I_{0} \cup I_{1} \cup I_{2} \cup \cdots \cup I_{n-2} \cup I_{n-1}
\end{align*}
From each $I_{i}$, choose a number $t_{i}$. We call the following set of ordered pairs a tagged partition
\begin{align*}
    \dot P = \{ \hspace{4pt} ( \hspace{4pt} [x_{i}, x_{i+1}), t_{i} \hspace{4pt} ) \hspace{4pt}\}_{i = 0}^{n-2} \hspace{10pt} \cup \hspace{10pt} \{ \hspace{4pt} ( \hspace{4pt} [x_{n-1}, x_{n}], t_{n-1} \hspace{4pt} ) \hspace{4pt} \}
\end{align*}
\end{definition}

\begin{definition}
The norm of a tagged partition is defined as
\begin{align*}
    \lvert \lvert \dot P \rvert \rvert = \max \{x_{1} - x_{0}, x_{2} - x_{1}, \cdots , x_{n-1} - x_{n-2}, x_{n} - x_{n-1}\}
\end{align*}
\end{definition}

\begin{definition}
A function $f$ on $I=[a, b]$ is said to be Riemann integrable on $[a, b]$ if there exists a real number $L$ such that for every $\epsilon > 0$ there exists a $\delta > 0$ satisfying the following
\begin{align*}
    &\text{whenever} \hspace{4pt} \dot P \hspace{4pt} \text{is a tagged partition of $[a, b]$}\\[2ex]
    &\text{if} \hspace{20pt} \lvert \lvert \dot P \rvert \rvert < \delta \hspace{20pt} \text{then} \hspace{20pt} \Big\lvert \sum_{i=0}^{n-1} f(t_{i})(x_{i+1} - x_{i}) - L \Big\rvert < \epsilon  
\end{align*}
For this course, we will use the following notation for $L$
\begin{align*}
    L = \int_{a}^{b} f(x) dx
\end{align*}
\end{definition}

\begin{example}
This is an example of a Riemann sum. There are infinitely many tagged partitions we could use for any example, all of which are merely an approximation of the integral of the function, except in the limit. We've chosen one that demonstrates the flexibility of these partitions. Notice that the widths of the rectangles are visibly different, and notice the visible difference in where $t_{i}$ is positioned for each interval. This particular partition for the function $f$ can be written as
\begin{align*}
    \dot P = \{ \hspace{4pt} ( \hspace{4pt} [x_{i}, x_{i+1}), t_{i} \hspace{4pt} ) \hspace{4pt} \}_{i = 0}^{6} \hspace{10pt} \cup \hspace{10pt} \{ \hspace{4pt} ( \hspace{4pt} [x_{7}, x_{8}], t_{7} \hspace{4pt} ) \hspace{4pt} \} \hspace{20pt} \text{where} \hspace{20pt} f(x) = \cos x \hspace{20pt} x \in [0, 1]  
\end{align*}
So, for our partition, we have the endpoints
\begin{align*}
    x_{0} = 0 \hspace{20pt} \text{and} \hspace{20pt} x_{8} = 1
\end{align*}
\resizebox{30em}{30em}{%
\begin{tikzpicture}[scale=\textwidth/4.2cm]
    % title and axes
    \node at (0.6, 1.2) {$f(x)=\cos x, \hspace{4pt} x \in [0, \pi]$};
    \draw (0, 0) -- (pi, 0);
    \draw (0, 0) -- (0, 1.4)
        node[above] {$f(x)$};
    \draw (0, 0) -- (0, -1);
    % graph
    \draw[black, very thick] plot[smooth] file {integrals_of_functions/python_generated_tables/cos_0_pi_riemann_sum.table};
    \draw[red, very thick, fill=yellow!30, opacity=0.5] (0, 0) 
        -- (pi/6, 0)
        -- (pi/6, {cos(pi/9 r)})
        -- (0, {cos(pi/9 r)})
        -- (0, 0);
    \node at (-0.1, -0.05) {$x_{0}$};
    \node at (pi/9, -0.3) {$t_{0}$};
    \node at (pi/6, -0.05) {$x_{1}$};
    \draw[black, dotted] (pi/9, -0.25) -- (pi/9, {cos(pi/9 r)});
    \draw[blue, fill=red] (pi/9, {cos(pi/9 r)}) circle (.25mm);
    \draw[red, very thick, fill=yellow!30, opacity=0.5] (pi/6, 0) 
        -- (pi/4, 0)
        -- (pi/4, {cos(pi/5 r)})
        -- (pi/6, {cos(pi/5 r)})
        -- (pi/6, 0);
    \node at (pi/5, -0.3) {$t_{1}$};
    \node at (pi/4, -0.05) {$x_{2}$};
    \draw[black, dotted] (pi/5, -0.25) -- (pi/5, {cos(pi/5 r)});
    \draw[blue, fill=red] (pi/5, {cos(pi/5 r)}) circle (.25mm);
    \draw[red, very thick, fill=yellow!30, opacity=0.5] (pi/4, 0) 
        -- (pi/3, 0)
        -- (pi/3, {cos(12*pi/38 r)})
        -- (pi/4, {cos(12*pi/38 r)})
        -- (pi/4, 0);
    \node at (12*pi/38, -0.3) {$t_{2}$};
    \node at (pi/3, -0.05) {$x_{3}$};
    \draw[black, dotted] (12*pi/38, -0.25) -- (12*pi/38, {cos(12*pi/38 r)});
    \draw[blue, fill=red] (12*pi/38, {cos(12*pi/38 r)}) circle (.25mm);
    \draw[red, very thick, fill=yellow!30, opacity=0.5] (pi/3, 0) 
        -- (pi/2, 0)
        -- (pi/2, {cos(12*pi/28 r)})
        -- (pi/3, {cos(12*pi/28 r)})
        -- (pi/3, 0);
    \node at (12*pi/28, -0.3) {$t_{3}$};
    \node at (8*pi/17, -0.05) {$x_{4}$};
    \draw[black, dotted] (12*pi/28, -0.25) -- (12*pi/28, {cos(12*pi/28 r)});
    \draw[blue, fill=red] (12*pi/28, {cos(12*pi/28 r)}) circle (.25mm);
    \draw[red, very thick, fill=yellow!30, opacity=0.5] (pi/2, 0) 
        -- (4*pi/7, 0)
        -- (4*pi/7, {cos(6*pi/11 r)})
        -- (pi/2, {cos(6*pi/11 r)})
        -- (pi/2, 0);
    \node at (6*pi/11, 0.3) {$t_{4}$};
    \node at (4*pi/7, 0.05) {$x_{5}$};
    \draw[black, dotted] (6*pi/11, 0.25) -- (6*pi/11, {cos(6*pi/11 r)});
    \draw[blue, fill=red] (6*pi/11, {cos(6*pi/11 r)}) circle (.25mm);
    \draw[red, very thick, fill=yellow!30, opacity=0.5] (4*pi/7, 0) 
        -- (3*pi/4, 0)
        -- (3*pi/4, {cos(2*pi/3 r)})
        -- (4*pi/7, {cos(2*pi/3 r)})
        -- (4*pi/7, 0);
    \node at (2*pi/3, 0.3) {$t_{5}$};
    \node at (3*pi/4, 0.05) {$x_{6}$};
    \draw[black, dotted] (2*pi/3, 0.25) -- (2*pi/3, {cos(2*pi/3 r)});
    \draw[blue, fill=red] (2*pi/3, {cos(2*pi/3 r)}) circle (.25mm);
    \draw[red, very thick, fill=yellow!30, opacity=0.5] (3*pi/4, 0) 
        -- (11*pi/12, 0)
        -- (11*pi/12, {cos(11*pi/12 r)})
        -- (3*pi/4, {cos(11*pi/12 r)})
        -- (3*pi/4, 0);
    \node at (11*pi/12, 0.3) {$t_{6}$};
    \node at (44*pi/49, 0.05) {$x_{7}$};
    \draw[black, dotted] (11*pi/12, 0.25) -- (11*pi/12, {cos(11*pi/12 r)});
    \draw[blue, fill=red] (11*pi/12, {cos(11*pi/12 r)}) circle (.25mm);
    \draw[red, very thick, fill=yellow!30, opacity=0.5] (11*pi/12, 0) 
        -- (pi, 0)
        -- (pi, {cos(22*pi/23 r)})
        -- (11*pi/12, {cos(22*pi/23 r)})
        -- (11*pi/12, 0);
    \node at (22*pi/23, 0.3) {$t_{7}$};
    \node at (pi, 0.05) {$x_{8}$};
    \draw[black, dotted] (22*pi/23, 0.25) -- (22*pi/23, {cos(22*pi/23 r)});
    \draw[blue, fill=red] (22*pi/23, {cos(22*pi/23 r)}) circle (.25mm);
\end{tikzpicture}
}
\begin{align*}
    &\text{The approximation can be computed with} \hspace{20pt} \sum_{i=0}^{7} f(t_{i})(x_{i+1} - x_{i})
\end{align*}
Taking a partition with uncountable infinitely many points between $0$ and $1$ is the key to computing the integral. The rectangles seen in this example each have an area: base times height. The difference $(x_{i+1} - x_{i})$ for each $i$ represents the base, while the function value at $t_{i}$ for each $i$ represents the height. So, the integral of our function $f$ ---the value of which we will discuss shortly--- can be expressed as the limit 
\begin{align*}
    \lim_{n \longrightarrow \infty} \sum_{i=0}^{n-1} \cos(t_{i}) (x_{i+1} - x_{i}) = \int_{0}^{1} \cos x dx = \sin x \hspace{4pt} x \in [0, 1]
\end{align*}
\label{integral_of_cosine}
\end{example}

\begin{theorem}
A function $f$ continuous on $[a, b]$ or continuous at all but a finite number of points along $[a, b]$ is integrable on $[a, b]$.
\label{monotone_continuous_functions_are_integrable}
\end{theorem}

Integration on the continuous functions mentioned in Theorem \ref{monotone_continuous_functions_are_integrable} will more times than not require us to use something referred to as antidifferentiation, as opposed to the computation of sums, using a result known as The Fundamental Theorem of Calculus, which we will get to later. For now, let's simply practice antidifferentiation on continuous functions and explore some properties of the Riemann integral. 

\begin{example}
The function $f(x) = \cos x$ is continuous on $[0, 1]$. Thus, for Example \ref{integral_of_cosine}, the antiderivative of $f$ is $g(x) = \sin x$.
\end{example}

\begin{example}
Take $f(x) = 1$ on some arbitrary domain $D$. The form of the integral on $f$ along this non-explicitly defined domain $D$ is referred to as the indefinite form of the integral. Meaning, the function domain is not bounded above or below by any specific real numbers. We will later discuss the difference between this indefinite form and what is known as the definite form of an integral, which we used in Example \ref{integral_of_cosine}. The domain is explicitly defined and bounded for cosine in that example, whereas the domain for $f$ in this example is not defined at all. More on this, later. In taking either form of the integral on a function $f$, the first question you should always ask yourself:
\begin{align*}
    &\text{The derivative of which function $g$ is equal to} \hspace{4pt} f?\\[2ex]
    &\text{Meaning, what is $g$, when} \hspace{4pt} \dfrac{dg}{dx} = f(x) \hspace{4pt} \text{?}
\end{align*}
Once you find $g$, \textbf{THAT} is the integral of $f$. With the indefinite form, we must consider the crucial detail of a real number (constant) as being part of the expression for our function $g$. Particularly, for our example, we know
\begin{align*}
f(x) = 1 \hspace{20pt} f(x) = 1 + 0
\end{align*}
and we know that the derivative of a constant is $0$ and the derivative of $x$ is $1$. So, when searching for the indefinite integral $g$, we not only must consider the `kernel' (the main part) of the function $f$, which in our case is $1$, we must also consider the implied $0$. 
Continuing with our example:
\begin{align*}
    \text{we know that} \hspace{20pt} \dfrac{d}{dx} (x+c) = \dfrac{d}{dx} x + \dfrac{d}{dx} c = 1 + 0 = 1 \hspace{20pt} \text{where} \hspace{4pt} c \in \mathbb{R}
\end{align*}
So, we have that $g(x) = x+c$, because $\dfrac{dg}{dx} = \dfrac{d}{dx}(x+c) = 1 + 0 = 1 = f(x)$. Additionally, because $f$ is continuous on $D$, we call $g$ an antiderivative of $f$. Thus, we have the indefinite integral
\begin{align*}
    g(x) = \int_{D} f(x)dx = \int_{D} 1 dx = x + c \hspace{20pt} \text{where $D$ is the domain of the function}
\end{align*}
which also happens to be an antiderivative. We could represent this integral without the $1$ under the integral sign, as follows
\begin{align*}
    g(x) = \int_{D} dx = x+c
\end{align*}
\end{example}

\begin{example}
Let's take the integral of $f(x) = x$. We know 
\begin{align*}
    \dfrac{d}{dx} \Big(\dfrac{x^{2}}{2} + c \Big) = \dfrac{d}{dx} \dfrac{x^{2}}{2} + \dfrac{d}{dx} c = \dfrac{2x}{2} + 0 = x
\end{align*}
So, $g(x) = \dfrac{x^{2}}{2} + c$ is the indefinite integral of $f$ and it also happens to be an antiderivative of $f$, since $f$ is continuous on $D$. The results are summarized below.
\begin{align*}
    \int_{D} f(x)dx = \int_{D} x dx  =  \dfrac{x^{2}}{2} + c = g(x)
\end{align*}
\end{example}

\begin{exercise}
Find the indefinite integral of the following
\begin{align*}
    f(x) = x^{n} \hspace{20pt} \text{where $n$ is a positive number} 
\end{align*}
\end{exercise}

\begin{exercise}
Find the indefinite integral of the following
\begin{align*}
    f(x) = x^{-n} \hspace{20pt} \text{where $n$ is a positive number}
\end{align*}
\end{exercise}

\begin{exercise}
Find the indefinite integral of the following
\begin{align*}
    f(x) = e^{x}
\end{align*}
\end{exercise}

\begin{exercise}
Find the indefinite integral of the following
\begin{align*}
    f(x) = \cos x
\end{align*}
\end{exercise}

\begin{exercise}
Find the indefinite integral of the following
\begin{align*}
    f(x) = \sin x
\end{align*}
\end{exercise}

\begin{theorem}
Following are some of the basic properties of the Riemann integral
\begin{align*}
    &\int_{D} c f(x) dx = c \int_{D} f(x) dx \hspace{20pt} \text{where} \hspace{4pt} c \in \mathbb{R}\\[2ex]
    &\int_{D} (f(x) + g(x)) dx = \int_{D} f(x) dx + \int_{D} g(x) dx\\[2ex]
    &\int_{D} (f(x) - g(x)) dx = \int_{D} f(x) dx - \int_{D} g(x) dx
\end{align*}
\end{theorem}

\begin{exercise}
Find the indefinite integral of the following
\begin{align*}
    f(x) = 1 + 3x
\end{align*}
\end{exercise}

\begin{exercise}
Find the indefinite integral of the following
\begin{align*}
    f(x) = x^{2} + 2x - 5
\end{align*}
\end{exercise}

\begin{exercise}
Find the indefinite integral of the following
\begin{align*}
    f(x) = 2 - x^{2}
\end{align*}
\end{exercise}

\begin{exercise}
Find the indefinite integral of the following
\begin{align*}
    f(x) = 1 + 2x^{3}
\end{align*}
\end{exercise}

\begin{exercise}
Find the indefinite integral of the following
\begin{align*}
    f(x) = \dfrac{1}{2}x - 1
\end{align*}
\end{exercise}

\begin{exercise}
Find the indefinite integral of the following
\begin{align*}
    f(x) = 3 - 2x
\end{align*}
\end{exercise}

\newpage
\section{The Fundamental Theorem of Calculus}

\begin{theorem}
For function $f$ as described in Theorem \ref{monotone_continuous_functions_are_integrable}, we have the indefinite integral of $f$ represented as
\begin{align*}
    g(x) = \int_{a}^{x} f(t) dt \hspace{20pt} x \in [a, b]
\end{align*}
where $a$ is referred to as a basepoint. On the interval $[a, b]$, we have $g$ is continuous, and on the interval $(a, b)$, save for possibly finitely many points, we have $g$ is differentiable, with
\begin{align*}
    g^{'}(z) = f(z) \hspace{20pt} \text{for all} \hspace{4pt} z \in (a, b) \hspace{20pt} \text{save possibly finitely many points where $f$ is discontinuous}
\end{align*}
When $f$ is continuous on the domain $[a, b]$, we call $g$ an antidervative of $f$. \label{FTC_1}
\end{theorem}

\begin{theorem}
For function $f$ as described in Theorem \ref{monotone_continuous_functions_are_integrable}, we have 
\begin{align*}
    g(b) - g(a) = \int_{a}^{b} f(x) dx \hspace{20pt} x \in [a, b]
\end{align*}
where $g$ is continuous on $[a, b]$. Also, $g$ is differentiable on $(a, b)$, save for finitely many points, with
\begin{align*}
    g^{'}(x) = f(x) \hspace{20pt} \text{for all} \hspace{4pt} x \in (a, b) \hspace{20pt} \text{save for possibly finitely many points where $f$ is discontinuous}
\end{align*}
When $f$ is continuous on $[a, b]$, $g$ is an antiderivative of $f$.
\end{theorem}

\begin{exercise}
Find the definite integral of the following
\begin{align*}
    f(x) = 1 + 3x \hspace{20pt} x \in [-1, 5]
\end{align*}
\end{exercise}

\begin{exercise}
Find the definite integral of the following
\begin{align*}
    f(x) = x^{2} + 2x - 5 \hspace{20pt} x \in [1, 4]
\end{align*}
\end{exercise}

\begin{exercise}
Find the definite integral of the following
\begin{align*}
    f(x) = 2 - x^{2} \hspace{20pt} x \in [0, 2]
\end{align*}
\end{exercise}

\begin{exercise}
Find the definite integral of the following
\begin{align*}
    f(x) = 1 + 2x^{3} \hspace{20pt} x \in [0, 5]
\end{align*}
\end{exercise}

\begin{exercise}
Find the definite integral of the following
\begin{align*}
    f(x) = \dfrac{1}{2}x - 1 \hspace{20pt} x \in [0, 3]
\end{align*}
\end{exercise}

\begin{exercise}
Find the definite integral of the following
\begin{align*}
    f(x) = 3 - 2x \hspace{20pt} x \in [-1, 3]
\end{align*}
\end{exercise}

\begin{theorem}
Following are more of the basic properties of the Riemann integral
\begin{align*}
    &\text{If} \hspace{4pt} f(x) \geq 0 \hspace{4pt} \text{for all $x \in D$} \hspace{20pt} \text{then} \hspace{20pt} \int_{D} f(x) dx \geq 0\\[2ex]
    &\text{If} \hspace{4pt} f(x) \leq g(x) \hspace{4pt} \text{for all $x \in D$} \hspace{20pt} \text{then} \hspace{20pt} \int_{D} f(x) dx \leq \int_{D} g(x) dx 
\end{align*}
\end{theorem}

\begin{example}
In many situations, we could make use of a substitution method to simplify our process of integration. Take the following
\begin{align*}
    f(x) = \sqrt{2x + 1} \hspace{20pt} x \in [0, 4]
\end{align*}
We have the definite integral represented as 
\begin{align*}
    g(x) = \int_{0}^{4} \sqrt{2x + 1} dx
\end{align*}
To make the job of integration easier, we could set $u(x) = 2x + 1$. This would imply the following
\begin{align*}
    \dfrac{du}{dx} = 2 \hspace{10pt} \Longleftrightarrow \hspace{10pt} \dfrac{du}{2} = dx \hspace{20pt} \text{and} \hspace{20pt} u(x) \in [1, 9]
\end{align*}
Thus, the integral can be rewritten from this substitution as
\begin{align*}
    g(x) = \int_{1}^{9} \dfrac{1}{2}\sqrt{u(x)} du = \int_{1}^{9} \dfrac{1}{2} \hspace{4pt} (u(x))^{1/2} \hspace{4pt} du = \dfrac{1}{3} (u(x))^{3/2} \hspace{20pt} u(x) \in [1, 9]
\end{align*}
The right hand side of the equality evaluates to $26/3$. However, if one wishes to revert back to expressions in terms of $x$, as opposed to $u(x)$, the numerically computation will be the same.
\begin{align*}
    g(x) &= \int_{1}^{9} \dfrac{1}{2}\sqrt{u(x)} du = \dfrac{1}{3} (u(x))^{3/2} \hspace{20pt} u(x) \in [1, 9]\\[2ex]
    &= \dfrac{1}{3} (\sqrt{2x + 1})^{3/2} \hspace{20pt} x \in [0, 4]\\[2ex]
    &= \dfrac{1}{3} (\sqrt{2(4) + 1})^{3/2} - \dfrac{1}{3} (\sqrt{2(0) + 1})^{3/2} = \dfrac{26}{3}
\end{align*}
\end{example}

\begin{example}
Consider the following indefinite integral
\begin{align*}
    g(x) = \int_{D} \cos^{3} x \sin x dx
\end{align*}
It looks tough, but we got this. Define
\begin{align*}
    u(x) = \cos x
\end{align*}
By differentiating $u$ with respect to $x$, we get
\begin{align*}
    \dfrac{du}{dx} = -\sin x \hspace{20pt} \Longleftrightarrow \hspace{20pt} -du = \sin x dx
\end{align*}
Thus, our indefinitie integral becomes
\begin{align*}
    g(x) &= \int_{D} -(u(x))^{3} du\\[2ex]
    &= \hspace{4pt} -\dfrac{1}{4} (u(x))^{4} + c\\[2ex]
    &= \hspace{4pt} -\dfrac{1}{4} \cos^{4} x + c
\end{align*}
\end{example}

\begin{exercise}
Find the indefinite integral of the following 
\begin{align*}
    f(x) = \dfrac{\sec^{2} \Big(\dfrac{1}{x}\Big)}{x^{2}}
\end{align*}
\end{exercise}

\begin{exercise}
Find the indefinite integral of the following 
\begin{align*}
    f(x) = x \sin(x^{2})
\end{align*}
\end{exercise}

\begin{exercise}
Find the indefinite integral of the following 
\begin{align*}
    f(x) = \dfrac{x}{(x^{2} + 1)^{2}}
\end{align*}
\end{exercise}

\begin{exercise}
Find the indefinite integral of the following 
\begin{align*}
    f(x) = e^{x} \sin (e^{x})
\end{align*}
\end{exercise}

\begin{exercise}
Find the indefinite integral of the following 
\begin{align*}
    f(x) = \dfrac{x}{x^{2} + 1}
\end{align*}
\end{exercise}

\begin{exercise}
Find the indefinite integral of the following 
\begin{align*}
    f(x) = \dfrac{(\ln x)^{2}}{x}
\end{align*}
\end{exercise}

\begin{exercise}
Find the indefinite integral of the following 
\begin{align*}
    f(x) = (1 + \tan x)^{5} \sec^{2} x
\end{align*}
\end{exercise}

\begin{exercise}
Find the indefinite integral of the following 
\begin{align*}
    f(x) = e^{x} \sin (e^{x})
\end{align*}
\end{exercise}

\begin{exercise}
Find the indefinite integral of the following 
\begin{align*}
    f(x) = \dfrac{\sin(\ln x)}{x}
\end{align*}
\end{exercise}

\begin{exercise}
Find the indefinite integral of the following 
\begin{align*}
    f(x) = \dfrac{\cos x}{\sin^{2} x}
\end{align*}
\end{exercise}

\begin{exercise}
Find the indefinite integral of the following 
\begin{align*}
    f(x) = \sqrt{\cot x} \csc^{2} x
\end{align*}
\end{exercise}

\begin{exercise}
Find the indefinite integral of the following 
\begin{align*}
    f(x) = \sec^{3} x \tan x
\end{align*}
\end{exercise}

\begin{exercise}
Find the indefinite integral of the following 
\begin{align*}
    f(x) = \dfrac{1+x}{1 + x^{2}}
\end{align*}
\end{exercise}

\begin{exercise}
Find the indefinite integral of the following 
\begin{align*}
    f(x) = \dfrac{x^{2}}{\sqrt{1 - x}}
\end{align*}
\end{exercise}

\begin{exercise}
Find the indefinite integral of the following 
\begin{align*}
    f(x) = \dfrac{x}{\sqrt[\leftroot{2}\uproot{2}4]{x + 2}}
\end{align*}
\end{exercise}

\begin{exercise}
Find the indefinite integral of the following 
\begin{align*}
    f(x) = x^{3} \sqrt{x^{2} + 1}
\end{align*}
\end{exercise}

\begin{exercise}
Find the definite integral of the following 
\begin{align*}
    f(x) = x^{2} (1 + 2x^{3})^{5} \hspace{20pt} x \in [0, 1]
\end{align*}
\end{exercise}

\begin{exercise}
Find the definite integral of the following 
\begin{align*}
    f(x) = \dfrac{e^{1/x}}{x^{2}} \hspace{20pt} x \in [1, 2]
\end{align*}
\end{exercise}

\begin{example}
Using Theorem \ref{FTC_1}, we can find the derivative of an indefinite integral. Take the following
\begin{align*}
    \int_{1}^{x^{4}} \sec t dt
\end{align*}
The function under the integral sign is continuous. Additionally, we have $x^{4}$ as our upper bound on the integral sign. Let's define $u(x) = x^{4}$. Our function $g$ can now be written as 
\begin{align*}
    g(x) = (v \circ u)(x) = \int_{1}^{u(x)} \sec t dt
\end{align*}
By The Fundamental Theorem of Calculus, along with The Chain Rule 
\begin{align*}
    \dfrac{dg}{dx} &= v^{'}(u(x)) \cdot u^{'}(x)\\[2ex] 
    &= \dfrac{d}{du} \Big( \int_{1}^{u(x)} \sec t dt \Big) \dfrac{du}{dx}\\[2ex]
    &= ( \sec u(x) ) \cdot 4x^{3}\\[2ex]
    &= 4x^{3} \sec x^{4} 
\end{align*}
\end{example}

\begin{exercise}
Find the derivative of $g$.
\begin{align*}
    g(x) = \int_{1}^{x} \dfrac{1}{t^{3} + 1} dt
\end{align*}
\end{exercise}